Update local simulation relation definition

src/opt/SimLocal.v
@@ -29,13 +29,13 @@ Require Import Semantics.
 Set Implicit Arguments.
 
 
-Inductive sim_local (lc_src lc_tgt:Local.t): Prop :=
+Inductive sim_local (pview:SimPromises.t) (lc_src lc_tgt:Local.t): Prop :=
 | sim_local_intro
     (TVIEW: TView.le lc_src.(Local.tview) lc_tgt.(Local.tview))
-    (PROMISES: SimPromises.sem SimPromises.bot SimPromises.bot lc_src.(Local.promises) lc_tgt.(Local.promises))
+    (PROMISES: SimPromises.sem pview SimPromises.bot lc_src.(Local.promises) lc_tgt.(Local.promises))
 .
 
-Program Instance sim_local_PreOrder: PreOrder sim_local.
+Program Instance sim_local_PreOrder: PreOrder (sim_local SimPromises.bot).
 Next Obligation.
   econs; try refl. apply SimPromises.sem_bot.
 Qed.
@@ -47,17 +47,23 @@ Next Obligation.
 Qed.
 
 Lemma sim_local_nonsynch_loc
-      loc lc_src lc_tgt
-      (SIM: sim_local lc_src lc_tgt)
+      pview loc lc_src lc_tgt
+      (SIM: sim_local pview lc_src lc_tgt)
       (NONSYNCH: Memory.nonsynch_loc loc lc_tgt.(Local.promises)):
   Memory.nonsynch_loc loc lc_src.(Local.promises).
 Proof.
-  inv SIM. eapply SimPromises.sem_bot_inv in PROMISES; auto. rewrite PROMISES. auto.
+  inv SIM. inv PROMISES.
+  ii. destruct msg. ss.
+  destruct (Memory.get loc t (Local.promises lc_tgt)) as [[? []]|] eqn:GET_TGT.
+  - exploit NONSYNCH; eauto. ss. i. subst.
+    exploit LE; eauto. intro X. rewrite GET in X. inv X.
+    unfold SimPromises.none_if. condtac; ss.
+  - exploit COMPLETE; eauto. rewrite SimPromises.bot_spec. ss.
 Qed.
 
 Lemma sim_local_nonsynch
-      lc_src lc_tgt
-      (SIM: sim_local lc_src lc_tgt)
+      pview lc_src lc_tgt
+      (SIM: sim_local pview lc_src lc_tgt)
       (NONSYNCH: Memory.nonsynch lc_tgt.(Local.promises)):
   Memory.nonsynch lc_src.(Local.promises).
 Proof.
@@ -65,33 +71,39 @@ Proof.
 Qed.
 
 Lemma sim_local_memory_bot
-      lc_src lc_tgt
-      (SIM: sim_local lc_src lc_tgt)
+      pview lc_src lc_tgt
+      (SIM: sim_local pview lc_src lc_tgt)
       (BOT: lc_tgt.(Local.promises) = Memory.bot):
   lc_src.(Local.promises) = Memory.bot.
 Proof.
-  inv SIM. eapply SimPromises.sem_bot_inv in PROMISES; auto. rewrite PROMISES. auto.
-Qed.
+  inv SIM. inv PROMISES. rewrite BOT in *.
+  apply Memory.ext. i. rewrite Memory.bot_get.
+  destruct (Memory.get loc ts (Local.promises lc_src)) as [[? []]|] eqn:GET_SRC; ss.
+  exploit COMPLETE; eauto.
+  - apply Memory.bot_get.
+  - rewrite SimPromises.bot_spec. ss.
+Qed.  
 
 Lemma sim_local_promise
+      pview
       lc1_src mem1_src
       lc1_tgt mem1_tgt
       lc2_tgt mem2_tgt
       loc from to val released kind
       (STEP_TGT: Local.promise_step lc1_tgt mem1_tgt loc from to val released lc2_tgt mem2_tgt kind)
-      (LOCAL1: sim_local lc1_src lc1_tgt)
+      (LOCAL1: sim_local pview lc1_src lc1_tgt)
       (MEM1: sim_memory mem1_src mem1_tgt)
       (WF1_SRC: Local.wf lc1_src mem1_src)
       (WF1_TGT: Local.wf lc1_tgt mem1_tgt)
       (MEM1_SRC: Memory.closed mem1_src)
       (MEM1_TGT: Memory.closed mem1_tgt):
   exists lc2_src mem2_src,
-    <<STEP_SRC: Local.promise_step lc1_src mem1_src loc from to val released lc2_src mem2_src kind>> /\
-    <<LOCAL2: sim_local lc2_src lc2_tgt>> /\
+    <<STEP_SRC: Local.promise_step lc1_src mem1_src loc from to val (SimPromises.none_if loc to pview released) lc2_src mem2_src (SimPromises.kind_transf loc to pview kind)>> /\
+    <<LOCAL2: sim_local pview lc2_src lc2_tgt>> /\
     <<MEM2: sim_memory mem2_src mem2_tgt>>.
 Proof.
   inv LOCAL1. inv STEP_TGT.
-  exploit SimPromises.promise_bot; eauto.
+  exploit SimPromises.promise; eauto.
   { apply WF1_SRC. }
   { apply WF1_TGT. }
   i. des.
@@ -99,19 +111,43 @@ Proof.
   exploit Memory.promise_future; try apply PROMISE_SRC; eauto.
   { apply WF1_SRC. }
   { apply WF1_SRC. }
+  { unfold SimPromises.none_if. condtac; ss. }
   i. des.
   esplits; eauto.
-  - econs; eauto.
+  - econs; eauto. unfold SimPromises.none_if. condtac; ss.
   - econs; eauto.
 Qed.
 
+Lemma sim_local_promise_bot
+      lc1_src mem1_src
+      lc1_tgt mem1_tgt
+      lc2_tgt mem2_tgt
+      loc from to val released kind
+      (STEP_TGT: Local.promise_step lc1_tgt mem1_tgt loc from to val released lc2_tgt mem2_tgt kind)
+      (LOCAL1: sim_local SimPromises.bot lc1_src lc1_tgt)
+      (MEM1: sim_memory mem1_src mem1_tgt)
+      (WF1_SRC: Local.wf lc1_src mem1_src)
+      (WF1_TGT: Local.wf lc1_tgt mem1_tgt)
+      (MEM1_SRC: Memory.closed mem1_src)
+      (MEM1_TGT: Memory.closed mem1_tgt):
+  exists lc2_src mem2_src,
+    <<STEP_SRC: Local.promise_step lc1_src mem1_src loc from to val released lc2_src mem2_src kind>> /\
+    <<LOCAL2: sim_local SimPromises.bot lc2_src lc2_tgt>> /\
+    <<MEM2: sim_memory mem2_src mem2_tgt>>.
+Proof.
+  exploit sim_local_promise; eauto.
+  unfold SimPromises.none_if. rewrite SimPromises.bot_spec.
+  rewrite SimPromises.kind_transf_bot. ss.
+Qed.
+
 Lemma sim_local_read
+      pview
       lc1_src mem1_src
       lc1_tgt mem1_tgt
       lc2_tgt
       loc ts val released_tgt ord_src ord_tgt
       (STEP_TGT: Local.read_step lc1_tgt mem1_tgt loc ts val released_tgt ord_tgt lc2_tgt)
-      (LOCAL1: sim_local lc1_src lc1_tgt)
+      (LOCAL1: sim_local pview lc1_src lc1_tgt)
       (MEM1: sim_memory mem1_src mem1_tgt)
       (WF1_SRC: Local.wf lc1_src mem1_src)
       (WF1_TGT: Local.wf lc1_tgt mem1_tgt)
@@ -121,7 +157,7 @@ Lemma sim_local_read
   exists released_src lc2_src,
     <<REL: View.opt_le released_src released_tgt>> /\
     <<STEP_SRC: Local.read_step lc1_src mem1_src loc ts val released_src ord_src lc2_src>> /\
-    <<LOCAL2: sim_local lc2_src lc2_tgt>>.
+    <<LOCAL2: sim_local pview lc2_src lc2_tgt>>.
 Proof.
   inv LOCAL1. inv STEP_TGT.
   exploit sim_memory_get; try apply MEM1; eauto. i. des.
@@ -133,6 +169,7 @@ Proof.
 Qed.
 
 Lemma sim_local_fulfill
+      pview
       lc1_src sc1_src mem1_src
       lc1_tgt sc1_tgt mem1_tgt
       lc2_tgt sc2_tgt
@@ -142,8 +179,9 @@ Lemma sim_local_fulfill
       (RELM_CLOSED: Memory.closed_opt_view releasedm_src mem1_src)
       (WF_RELM_TGT: View.opt_wf releasedm_tgt)
       (ORD: Ordering.le ord_src ord_tgt)
+      (PVIEW: SimPromises.mem loc to pview = false \/ Ordering.le ord_tgt Ordering.plain)
       (STEP_TGT: fulfill_step lc1_tgt sc1_tgt loc from to val releasedm_tgt released ord_tgt lc2_tgt sc2_tgt)
-      (LOCAL1: sim_local lc1_src lc1_tgt)
+      (LOCAL1: sim_local pview lc1_src lc1_tgt)
       (SC1: TimeMap.le sc1_src sc1_tgt)
       (MEM1: sim_memory mem1_src mem1_tgt)
       (WF1_SRC: Local.wf lc1_src mem1_src)
@@ -153,10 +191,11 @@ Lemma sim_local_fulfill
       (MEM1_SRC: Memory.closed mem1_src)
       (MEM1_TGT: Memory.closed mem1_tgt):
   exists lc2_src sc2_src,
-    <<STEP_SRC: fulfill_step lc1_src sc1_src loc from to val releasedm_src released ord_src lc2_src sc2_src>> /\
-    <<LOCAL2: sim_local lc2_src lc2_tgt>> /\
+    <<STEP_SRC: fulfill_step lc1_src sc1_src loc from to val releasedm_src (SimPromises.none_if loc to pview released) ord_src lc2_src sc2_src>> /\
+    <<LOCAL2: sim_local (SimPromises.unset loc to pview) lc2_src lc2_tgt>> /\
     <<SC2: TimeMap.le sc2_src sc2_tgt>>.
 Proof.
+  guardH PVIEW.
   inv STEP_TGT.
   assert (RELT_LE:
    View.opt_le
@@ -171,21 +210,117 @@ Proof.
   { unfold TView.write_released. condtac; econs.
     repeat (try condtac; viewtac; try apply WF1_SRC).
   }
-  exploit SimPromises.remove_bot; try exact REMOVE;
+  exploit SimPromises.remove; try exact REMOVE;
     try exact MEM1; try apply LOCAL1; eauto.
   { apply WF1_SRC. }
   { apply WF1_TGT. }
   { apply WF1_TGT. }
   i. des. esplits.
   - econs; eauto.
-    eapply TViewFacts.writable_mon; eauto. apply LOCAL1.
+    + unfold SimPromises.none_if. condtac.
+      * unguardH PVIEW. des; ss. unfold TView.write_released. condtac; [|refl].
+        destruct ord_src, ord_tgt; inv ORD; inv PVIEW; inv COND0.
+      * etrans; eauto.
+    + unfold SimPromises.none_if. condtac; viewtac.
+    + eapply TViewFacts.writable_mon; try exact WRITABLE; eauto. apply LOCAL1.
   - econs; eauto. s. apply TViewFacts.write_tview_mon; auto.
     + apply LOCAL1.
     + apply WF1_TGT.
   - ss.
 Qed.
 
+Lemma sim_local_fulfill_bot
+      lc1_src sc1_src mem1_src
+      lc1_tgt sc1_tgt mem1_tgt
+      lc2_tgt sc2_tgt
+      loc from to val releasedm_src releasedm_tgt released ord_src ord_tgt
+      (RELM_LE: View.opt_le releasedm_src releasedm_tgt)
+      (RELM_WF: View.opt_wf releasedm_src)
+      (RELM_CLOSED: Memory.closed_opt_view releasedm_src mem1_src)
+      (WF_RELM_TGT: View.opt_wf releasedm_tgt)
+      (ORD: Ordering.le ord_src ord_tgt)
+      (STEP_TGT: fulfill_step lc1_tgt sc1_tgt loc from to val releasedm_tgt released ord_tgt lc2_tgt sc2_tgt)
+      (LOCAL1: sim_local SimPromises.bot lc1_src lc1_tgt)
+      (SC1: TimeMap.le sc1_src sc1_tgt)
+      (MEM1: sim_memory mem1_src mem1_tgt)
+      (WF1_SRC: Local.wf lc1_src mem1_src)
+      (WF1_TGT: Local.wf lc1_tgt mem1_tgt)
+      (SC1_SRC: Memory.closed_timemap sc1_src mem1_src)
+      (SC1_TGT: Memory.closed_timemap sc1_tgt mem1_tgt)
+      (MEM1_SRC: Memory.closed mem1_src)
+      (MEM1_TGT: Memory.closed mem1_tgt):
+  exists lc2_src sc2_src,
+    <<STEP_SRC: fulfill_step lc1_src sc1_src loc from to val releasedm_src released ord_src lc2_src sc2_src>> /\
+    <<LOCAL2: sim_local SimPromises.bot lc2_src lc2_tgt>> /\
+    <<SC2: TimeMap.le sc2_src sc2_tgt>>.
+Proof.
+  exploit sim_local_fulfill; eauto.
+  { rewrite SimPromises.bot_spec. intuition. }
+  i. des. esplits; eauto.
+  rewrite SimPromises.unset_bot in *; ss.
+Qed.
+
 Lemma sim_local_write
+      pview
+      lc1_src sc1_src mem1_src
+      lc1_tgt sc1_tgt mem1_tgt
+      lc2_tgt sc2_tgt mem2_tgt
+      loc from to val releasedm_src releasedm_tgt released_tgt ord_src ord_tgt kind
+      (RELM_LE: View.opt_le releasedm_src releasedm_tgt)
+      (RELM_SRC_WF: View.opt_wf releasedm_src)
+      (RELM_SRC_CLOSED: Memory.closed_opt_view releasedm_src mem1_src)
+      (RELM_TGT_WF: View.opt_wf releasedm_tgt)
+      (RELM_TGT_CLOSED: Memory.closed_opt_view releasedm_tgt mem1_tgt)
+      (ORD: Ordering.le ord_src ord_tgt)
+      (PVIEW: SimPromises.mem loc to pview = false \/
+              Ordering.le ord_tgt Ordering.plain \/
+              Ordering.le Ordering.strong_relaxed ord_tgt)
+      (STEP_TGT: Local.write_step lc1_tgt sc1_tgt mem1_tgt loc from to val releasedm_tgt released_tgt ord_tgt lc2_tgt sc2_tgt mem2_tgt kind)
+      (LOCAL1: sim_local pview lc1_src lc1_tgt)
+      (SC1: TimeMap.le sc1_src sc1_tgt)
+      (MEM1: sim_memory mem1_src mem1_tgt)
+      (WF1_SRC: Local.wf lc1_src mem1_src)
+      (WF1_TGT: Local.wf lc1_tgt mem1_tgt)
+      (SC1_SRC: Memory.closed_timemap sc1_src mem1_src)
+      (SC1_TGT: Memory.closed_timemap sc1_tgt mem1_tgt)
+      (MEM1_SRC: Memory.closed mem1_src)
+      (MEM1_TGT: Memory.closed mem1_tgt):
+  exists released_src lc2_src sc2_src mem2_src,
+    <<STEP_SRC: Local.write_step lc1_src sc1_src mem1_src loc from to val releasedm_src
+                                 released_src
+                                 ord_src lc2_src sc2_src mem2_src
+                                 (SimPromises.kind_transf loc to pview kind)>> /\
+    <<REL2: View.opt_le released_src released_tgt>> /\
+    <<LOCAL2: sim_local (SimPromises.unset loc to pview) lc2_src lc2_tgt>> /\
+    <<SC2: TimeMap.le sc2_src sc2_tgt>> /\
+    <<MEM2: sim_memory mem2_src mem2_tgt>>.
+Proof.
+  guardH PVIEW.
+  exploit write_promise_fulfill; eauto. i. des.
+  exploit Local.promise_step_future; eauto. i. des.
+  exploit sim_local_promise; eauto. i. des.
+  exploit Local.promise_step_future; eauto. i. des.
+  exploit sim_local_fulfill; try apply STEP2;
+    try apply LOCAL2; try apply MEM2; eauto.
+  { eapply Memory.future_closed_opt_view; eauto. }
+  { unguardH PVIEW. des; intuition.
+    admit. (* it's add; so pview = false *)
+  }
+  i. des.
+  exploit promise_fulfill_write; try exact STEP_SRC; try exact STEP_SRC0; eauto.
+  { i. exploit ORD0; eauto.
+    - etrans; eauto.
+    - i. des. splits; auto.
+      + eapply sim_local_nonsynch_loc; eauto.
+      + subst. ss.
+  }
+  i. des. subst. esplits; eauto.
+  - apply TViewFacts.write_released_mon; ss;
+      try apply LOCAL1; try apply WF1_TGT.
+  - etrans; eauto.
+Admitted.
+
+Lemma sim_local_write_bot
       lc1_src sc1_src mem1_src
       lc1_tgt sc1_tgt mem1_tgt
       lc2_tgt sc2_tgt mem2_tgt
@@ -197,7 +332,7 @@ Lemma sim_local_write
       (RELM_TGT_CLOSED: Memory.closed_opt_view releasedm_tgt mem1_tgt)
       (ORD: Ordering.le ord_src ord_tgt)
       (STEP_TGT: Local.write_step lc1_tgt sc1_tgt mem1_tgt loc from to val releasedm_tgt released_tgt ord_tgt lc2_tgt sc2_tgt mem2_tgt kind)
-      (LOCAL1: sim_local lc1_src lc1_tgt)
+      (LOCAL1: sim_local SimPromises.bot lc1_src lc1_tgt)
       (SC1: TimeMap.le sc1_src sc1_tgt)
       (MEM1: sim_memory mem1_src mem1_tgt)
       (WF1_SRC: Local.wf lc1_src mem1_src)
@@ -207,29 +342,24 @@ Lemma sim_local_write
       (MEM1_SRC: Memory.closed mem1_src)
       (MEM1_TGT: Memory.closed mem1_tgt):
   exists released_src lc2_src sc2_src mem2_src,
-    <<STEP_SRC: Local.write_step lc1_src sc1_src mem1_src loc from to val releasedm_src released_src ord_src lc2_src sc2_src mem2_src kind>> /\
+    <<STEP_SRC: Local.write_step lc1_src sc1_src mem1_src loc from to val releasedm_src
+                                 released_src
+                                 ord_src lc2_src sc2_src mem2_src
+                                 kind>> /\
     <<REL2: View.opt_le released_src released_tgt>> /\
-    <<LOCAL2: sim_local lc2_src lc2_tgt>> /\
+    <<LOCAL2: sim_local SimPromises.bot lc2_src lc2_tgt>> /\
     <<SC2: TimeMap.le sc2_src sc2_tgt>> /\
     <<MEM2: sim_memory mem2_src mem2_tgt>>.
 Proof.
-  exploit write_promise_fulfill; eauto. i. des.
-  exploit Local.promise_step_future; eauto. i. des.
-  exploit sim_local_promise; eauto. i. des.
-  exploit Local.promise_step_future; eauto. i. des.
-  exploit sim_local_fulfill; try apply STEP2;
-    try apply LOCAL2; try apply MEM2; eauto.
-  { eapply Memory.future_closed_opt_view; eauto. }
-  i. des.
-  exploit promise_fulfill_write; try exact STEP_SRC; try exact STEP_SRC0; eauto.
-  { i. exploit ORD0; eauto.
-    - etrans; eauto.
-    - i. des. splits; auto. eapply sim_local_nonsynch_loc; eauto.
-  }
-  i. des. esplits; eauto. etrans; eauto.
+  hexploit sim_local_write; eauto.
+  { rewrite SimPromises.bot_spec. intuition. }
+  i. des. esplits; eauto.
+  - rewrite SimPromises.kind_transf_bot in *. eauto.
+  - rewrite SimPromises.unset_bot in *; ss.
 Qed.
 
 Lemma sim_local_update
+      pview
       lc1_src sc1_src mem1_src
       lc1_tgt sc1_tgt mem1_tgt
       lc2_tgt
@@ -238,7 +368,48 @@ Lemma sim_local_update
       from2 to2 val2 released2_tgt ord2_src ord2_tgt kind
       (STEP1_TGT: Local.read_step lc1_tgt mem1_tgt loc ts1 val1 released1_tgt ord1_tgt lc2_tgt)
       (STEP2_TGT: Local.write_step lc2_tgt sc1_tgt mem1_tgt loc from2 to2 val2 released1_tgt released2_tgt ord2_tgt lc3_tgt sc3_tgt mem3_tgt kind)
-      (LOCAL1: sim_local lc1_src lc1_tgt)
+      (LOCAL1: sim_local pview lc1_src lc1_tgt)
+      (SC1: TimeMap.le sc1_src sc1_tgt)
+      (MEM1: sim_memory mem1_src mem1_tgt)
+      (WF1_SRC: Local.wf lc1_src mem1_src)
+      (WF1_TGT: Local.wf lc1_tgt mem1_tgt)
+      (SC1_SRC: Memory.closed_timemap sc1_src mem1_src)
+      (SC1_TGT: Memory.closed_timemap sc1_tgt mem1_tgt)
+      (MEM1_SRC: Memory.closed mem1_src)
+      (MEM1_TGT: Memory.closed mem1_tgt)
+      (ORD1: Ordering.le ord1_src ord1_tgt)
+      (ORD2: Ordering.le ord2_src ord2_tgt)
+      (PVIEW: SimPromises.mem loc to2 pview = false \/
+              Ordering.le ord2_tgt Ordering.plain \/
+              Ordering.le Ordering.strong_relaxed ord2_tgt):
+  exists released1_src released2_src lc2_src lc3_src sc3_src mem3_src,
+    <<REL1: View.opt_le released1_src released1_tgt>> /\
+    <<REL2: View.opt_le released2_src released2_tgt>> /\
+    <<STEP1_SRC: Local.read_step lc1_src mem1_src loc ts1 val1 released1_src ord1_src lc2_src>> /\
+    <<STEP2_SRC: Local.write_step lc2_src sc1_src mem1_src loc from2 to2 val2 released1_src released2_src ord2_src lc3_src sc3_src mem3_src
+                                  (SimPromises.kind_transf loc to2 pview kind)>> /\
+    <<LOCAL3: sim_local (SimPromises.unset loc to2 pview) lc3_src lc3_tgt>> /\
+    <<SC3: TimeMap.le sc3_src sc3_tgt>> /\
+    <<MEM3: sim_memory mem3_src mem3_tgt>>.
+Proof.
+  guardH PVIEW.
+  exploit Local.read_step_future; eauto. i. des.
+  exploit sim_local_read; eauto. i. des.
+  exploit Local.read_step_future; eauto. i. des.
+  hexploit sim_local_write; eauto. i. des.
+  esplits; eauto.
+Qed.
+
+Lemma sim_local_update_bot
+      lc1_src sc1_src mem1_src
+      lc1_tgt sc1_tgt mem1_tgt
+      lc2_tgt
+      lc3_tgt sc3_tgt mem3_tgt
+      loc ts1 val1 released1_tgt ord1_src ord1_tgt
+      from2 to2 val2 released2_tgt ord2_src ord2_tgt kind
+      (STEP1_TGT: Local.read_step lc1_tgt mem1_tgt loc ts1 val1 released1_tgt ord1_tgt lc2_tgt)
+      (STEP2_TGT: Local.write_step lc2_tgt sc1_tgt mem1_tgt loc from2 to2 val2 released1_tgt released2_tgt ord2_tgt lc3_tgt sc3_tgt mem3_tgt kind)
+      (LOCAL1: sim_local SimPromises.bot lc1_src lc1_tgt)
       (SC1: TimeMap.le sc1_src sc1_tgt)
       (MEM1: sim_memory mem1_src mem1_tgt)
       (WF1_SRC: Local.wf lc1_src mem1_src)
@@ -254,25 +425,26 @@ Lemma sim_local_update
     <<REL2: View.opt_le released2_src released2_tgt>> /\
     <<STEP1_SRC: Local.read_step lc1_src mem1_src loc ts1 val1 released1_src ord1_src lc2_src>> /\
     <<STEP2_SRC: Local.write_step lc2_src sc1_src mem1_src loc from2 to2 val2 released1_src released2_src ord2_src lc3_src sc3_src mem3_src kind>> /\
-    <<LOCAL3: sim_local lc3_src lc3_tgt>> /\
+    <<LOCAL3: sim_local SimPromises.bot lc3_src lc3_tgt>> /\
     <<SC3: TimeMap.le sc3_src sc3_tgt>> /\
     <<MEM3: sim_memory mem3_src mem3_tgt>>.
 Proof.
   exploit Local.read_step_future; eauto. i. des.
   exploit sim_local_read; eauto. i. des.
   exploit Local.read_step_future; eauto. i. des.
-  hexploit sim_local_write; eauto. i. des.
+  hexploit sim_local_write_bot; eauto. i. des.
   esplits; eauto.
 Qed.
 
 Lemma sim_local_fence
+      pview
       lc1_src sc1_src mem1_src
       lc1_tgt sc1_tgt mem1_tgt
       lc2_tgt sc2_tgt
       ordr_src ordw_src
       ordr_tgt ordw_tgt
       (STEP_TGT: Local.fence_step lc1_tgt sc1_tgt ordr_tgt ordw_tgt lc2_tgt sc2_tgt)
-      (LOCAL1: sim_local lc1_src lc1_tgt)
+      (LOCAL1: sim_local pview lc1_src lc1_tgt)
       (SC1: TimeMap.le sc1_src sc1_tgt)
       (MEM1: sim_memory mem1_src mem1_tgt)
       (WF1_SRC: Local.wf lc1_src mem1_src)
@@ -281,7 +453,7 @@ Lemma sim_local_fence
       (ORDW: Ordering.le ordw_src ordw_tgt):
   exists lc2_src sc2_src,
     <<STEP_SRC: Local.fence_step lc1_src sc1_src ordr_src ordw_src lc2_src sc2_src>> /\
-    <<LOCAL2: sim_local lc2_src lc2_tgt>> /\
+    <<LOCAL2: sim_local pview lc2_src lc2_tgt>> /\
     <<SC2: TimeMap.le sc2_src sc2_tgt>>.
 Proof.
   inv STEP_TGT. esplits; eauto.
@@ -311,14 +483,14 @@ Lemma sim_local_program_step
       (MEM1_SRC: Memory.closed th1_src.(Thread.memory))
       (MEM1_TGT: Memory.closed th1_tgt.(Thread.memory))
       (STATE: th1_src.(Thread.state) = th1_tgt.(Thread.state))
-      (LOCAL: sim_local th1_src.(Thread.local) th1_tgt.(Thread.local))
+      (LOCAL: sim_local SimPromises.bot th1_src.(Thread.local) th1_tgt.(Thread.local))
       (SC: TimeMap.le th1_src.(Thread.sc) th1_tgt.(Thread.sc))
       (MEM: sim_memory th1_src.(Thread.memory) th1_tgt.(Thread.memory)):
   exists e_src th2_src,
     <<STEP_SRC: @Thread.program_step lang e_src th1_src th2_src>> /\
     <<EVENT: ThreadEvent.get_event e_src = ThreadEvent.get_event e_tgt>> /\
     <<STATE: th2_src.(Thread.state) = th2_tgt.(Thread.state)>> /\
-    <<LOCAL: sim_local th2_src.(Thread.local) th2_tgt.(Thread.local)>> /\
+    <<LOCAL: sim_local SimPromises.bot th2_src.(Thread.local) th2_tgt.(Thread.local)>> /\
     <<SC: TimeMap.le th2_src.(Thread.sc) th2_tgt.(Thread.sc)>> /\
     <<MEM: sim_memory th2_src.(Thread.memory) th2_tgt.(Thread.memory)>>.
 Proof.
@@ -327,12 +499,12 @@ Proof.
   - esplits; (try by econs; [|econs 1]; eauto); ss.
   - exploit sim_local_read; eauto; try refl. i. des.
     esplits; (try by econs; [|econs 2]; eauto); ss.
-  - hexploit sim_local_write; eauto; try refl; try by viewtac. i. des.
+  - hexploit sim_local_write_bot; eauto; try refl; try by viewtac. i. des.
     esplits; (try by econs; [|econs 3]; eauto); ss.
   - exploit Local.read_step_future; eauto. i. des.
     exploit sim_local_read; eauto; try refl. i. des.
     exploit Local.read_step_future; eauto. i. des.
-    hexploit sim_local_write; eauto; try refl; try by viewtac. i. des.
+    hexploit sim_local_write_bot; eauto; try refl; try by viewtac. i. des.
     esplits; (try by econs; [|econs 4]; eauto); ss.
   - exploit sim_local_fence; eauto; try refl. i. des.
     esplits; (try by econs; [|econs 5]; eauto); ss.
